src/lib.rs
@@ -8,7 +8,7 @@ use std::array::TryFromSliceError;
 
 use subtle::{Choice, ConstantTimeEq};
 
-pub use field::FieldElement;
+use field::FieldElement;
 mod field;
 
 mod traits;
@@ -20,12 +20,16 @@ pub mod constants;
 #[derive(Copy, Clone, Eq, Hash)]
 pub struct CompressedRistretto(pub [u8; 32]);
 
+#[hax_lib::attributes]
+#[hax_lib::fstar::verification_status(lax)]
 impl PartialEq for CompressedRistretto {
     fn eq(&self, other: &Self) -> bool {
         self.0.ct_eq(&other.0).into()
     }
 }
 
+#[hax_lib::attributes]
+#[hax_lib::fstar::verification_status(lax)]
 impl ConstantTimeEq for CompressedRistretto {
     fn ct_eq(&self, other: &CompressedRistretto) -> Choice {
         self.as_bytes().ct_eq(other.as_bytes())
@@ -33,6 +37,7 @@ impl ConstantTimeEq for CompressedRistretto {
 }
 
 #[hax_lib::attributes]
+#[hax_lib::fstar::verification_status(lax)]
 impl CompressedRistretto {
     /// Copy the bytes of this `CompressedRistretto`.
     pub const fn to_bytes(&self) -> [u8; 32] {
@@ -50,8 +55,7 @@ impl CompressedRistretto {
     ///
     /// Returns [`TryFromSliceError`] if the input `bytes` slice does not have
     /// a length of 32.
-    #[hax_lib::requires(bytes.len() == 32)]
-    #[hax_lib::ensures(|r| r.is_ok())]
+    #[hax_lib::requires(fstar!("True"))]
     pub fn from_slice(bytes: &[u8]) -> Result<CompressedRistretto, TryFromSliceError> {
         bytes.try_into().map(CompressedRistretto)
     }
@@ -92,6 +96,8 @@ impl Default for CompressedRistretto {
     }
 }
 
+#[hax_lib::attributes]
+#[hax_lib::fstar::verification_status(lax)]
 impl TryFrom<&[u8]> for CompressedRistretto {
     type Error = TryFromSliceError;
 
@@ -103,7 +109,6 @@ impl TryFrom<&[u8]> for CompressedRistretto {
 mod decompress {
     use super::*;
 
-    #[hax_lib::attributes]
     pub(super) fn step_1(repr: &CompressedRistretto) -> (Choice, Choice, FieldElement) {
         // Step 1. Check s for validity:
         // 1.a) s must be 32 bytes
@@ -117,7 +122,6 @@ mod decompress {
         (s_encoding_is_canonical, s_is_negative, s)
     }
 
-    #[hax_lib::attributes]
     pub(super) fn step_2(s: FieldElement) -> (Choice, Choice, Choice, RistrettoPoint) {
         // Step 2.  Compute (X:Y:Z:T).
         let one = FieldElement::ONE;
