proofs/fstar/extraction/Ristretto255.Bundle.fst
@@ -6,882 +6,335 @@ open Core_models
 let _ =
   (* This module has implicit dependencies, here we make them explicit. *)
   (* The implicit dependencies arise from typeclasses instances. *)
+  let open Ristretto255.Field in
   let open Ristretto255.Traits in
   let open Subtle in
   ()
 
-type t_FieldElement = | FieldElement : t_Array u64 (mk_usize 5) -> t_FieldElement
+/// A compressed Ristretto255 point.
+type t_CompressedRistretto =
+  | CompressedRistretto : t_Array u8 (mk_usize 32) -> t_CompressedRistretto
 
-/// Edwards `d` value, equal to `-121665/121666 mod p`.
-let v_EDWARDS_D: t_FieldElement =
-  FieldElement
-  (let list =
-      [
-        mk_u64 929955233495203;
-        mk_u64 466365720129213;
-        mk_u64 1662059464998953;
-        mk_u64 2033849074728123;
-        mk_u64 1442794654840575
-      ]
-    in
-    FStar.Pervasives.assert_norm (Prims.eq2 (List.Tot.length list) 5);
-    Rust_primitives.Hax.array_of_list 5 list)
-  <:
-  t_FieldElement
-
-/// Precomputed value of one of the square roots of -1 (mod p).
-let v_SQRT_M1: t_FieldElement =
-  FieldElement
-  (let list =
-      [
-        mk_u64 1718705420411056;
-        mk_u64 234908883556509;
-        mk_u64 2233514472574048;
-        mk_u64 2117202627021982;
-        mk_u64 765476049583133
-      ]
-    in
-    FStar.Pervasives.assert_norm (Prims.eq2 (List.Tot.length list) 5);
-    Rust_primitives.Hax.array_of_list 5 list)
-  <:
-  t_FieldElement
-
-let impl_11: Core_models.Clone.t_Clone t_FieldElement =
+let impl_3: Core_models.Clone.t_Clone t_CompressedRistretto =
   { f_clone = (fun x -> x); f_clone_pre = (fun _ -> True); f_clone_post = (fun _ _ -> True) }
 
 [@@ FStar.Tactics.Typeclasses.tcinstance]
 assume
-val impl_12': Core_models.Marker.t_Copy t_FieldElement
+val impl_2': Core_models.Marker.t_Copy t_CompressedRistretto
 
 unfold
-let impl_12 = impl_12'
+let impl_2 = impl_2'
 
 [@@ FStar.Tactics.Typeclasses.tcinstance]
 assume
-val impl_13': Core_models.Fmt.t_Debug t_FieldElement
+val impl_5': Core_models.Hash.t_Hash t_CompressedRistretto
 
 unfold
-let impl_13 = impl_13'
+let impl_5 = impl_5'
+
+#push-options "--admit_smt_queries true"
+
+[@@ FStar.Tactics.Typeclasses.tcinstance]
+let impl_6: Core_models.Cmp.t_PartialEq t_CompressedRistretto t_CompressedRistretto =
+  {
+    f_eq_pre = (fun (self: t_CompressedRistretto) (other: t_CompressedRistretto) -> true);
+    f_eq_post
+    =
+    (fun (self: t_CompressedRistretto) (other: t_CompressedRistretto) (out: bool) -> true);
+    f_eq
+    =
+    fun (self: t_CompressedRistretto) (other: t_CompressedRistretto) ->
+      Core_models.Convert.f_into #Subtle.t_Choice
+        #bool
+        #FStar.Tactics.Typeclasses.solve
+        (Subtle.f_ct_eq #(t_Slice u8)
+            #FStar.Tactics.Typeclasses.solve
+            (self._0 <: t_Slice u8)
+            (other._0 <: t_Slice u8)
+          <:
+          Subtle.t_Choice)
+  }
+
+#pop-options
 
 [@@ FStar.Tactics.Typeclasses.tcinstance]
 assume
-val impl_14': Core_models.Marker.t_StructuralPartialEq t_FieldElement
+val impl_4': Core_models.Cmp.t_Eq t_CompressedRistretto
 
 unfold
-let impl_14 = impl_14'
+let impl_4 = impl_4'
+
+/// Copy the bytes of this `CompressedRistretto`.
+let impl_8__to_bytes (self: t_CompressedRistretto) : t_Array u8 (mk_usize 32) = self._0
+
+/// View this `CompressedRistretto` as an array of bytes.
+let impl_8__as_bytes (self: t_CompressedRistretto) : t_Array u8 (mk_usize 32) = self._0
+
+#push-options "--admit_smt_queries true"
 
 [@@ FStar.Tactics.Typeclasses.tcinstance]
-assume
-val impl_15': Core_models.Cmp.t_PartialEq t_FieldElement t_FieldElement
+let impl_7: Subtle.t_ConstantTimeEq t_CompressedRistretto =
+  {
+    f_ct_eq_pre = (fun (self: t_CompressedRistretto) (other: t_CompressedRistretto) -> true);
+    f_ct_eq_post
+    =
+    (fun (self: t_CompressedRistretto) (other: t_CompressedRistretto) (out: Subtle.t_Choice) -> true
+    );
+    f_ct_eq
+    =
+    fun (self: t_CompressedRistretto) (other: t_CompressedRistretto) ->
+      Subtle.f_ct_eq #(t_Slice u8)
+        #FStar.Tactics.Typeclasses.solve
+        (impl_8__as_bytes self <: t_Slice u8)
+        (impl_8__as_bytes other <: t_Slice u8)
+  }
 
-unfold
-let impl_15 = impl_15'
+#pop-options
+
+/// Construct a `CompressedRistretto` from a slice of bytes.
+/// # Errors
+/// Returns [`TryFromSliceError`] if the input `bytes` slice does not have
+/// a length of 32.
+let impl_8__from_slice (bytes: t_Slice u8)
+    : Prims.Pure
+      (Core_models.Result.t_Result t_CompressedRistretto Core_models.Array.t_TryFromSliceError)
+      (requires True)
+      (fun _ -> Prims.l_True) =
+  Core_models.Result.impl__map #(t_Array u8 (mk_usize 32))
+    #Core_models.Array.t_TryFromSliceError
+    #t_CompressedRistretto
+    (Core_models.Convert.f_try_into #(t_Slice u8)
+        #(t_Array u8 (mk_usize 32))
+        #FStar.Tactics.Typeclasses.solve
+        bytes
+      <:
+      Core_models.Result.t_Result (t_Array u8 (mk_usize 32)) Core_models.Array.t_TryFromSliceError)
+    CompressedRistretto
 
 [@@ FStar.Tactics.Typeclasses.tcinstance]
-assume
-val impl_16': Core_models.Cmp.t_Eq t_FieldElement
-
-unfold
-let impl_16 = impl_16'
-
-[@@ FStar.Tactics.Typeclasses.tcinstance]
-let impl: Ristretto255.Traits.t_Identity t_FieldElement =
+let impl: Ristretto255.Traits.t_Identity t_CompressedRistretto =
   {
     f_identity_pre = (fun (_: Prims.unit) -> true);
-    f_identity_post = (fun (_: Prims.unit) (out: t_FieldElement) -> true);
+    f_identity_post = (fun (_: Prims.unit) (out: t_CompressedRistretto) -> true);
     f_identity
     =
     fun (_: Prims.unit) ->
-      FieldElement (Rust_primitives.Hax.repeat (mk_u64 0) (mk_usize 5)) <: t_FieldElement
-  }
-
-[@@ FStar.Tactics.Typeclasses.tcinstance]
-let impl_2: Core_models.Ops.Arith.t_Add t_FieldElement t_FieldElement =
-  {
-    f_Output = t_FieldElement;
-    f_add_pre = (fun (self: t_FieldElement) (rhs: t_FieldElement) -> true);
-    f_add_post = (fun (self: t_FieldElement) (rhs: t_FieldElement) (out1: t_FieldElement) -> true);
-    f_add
-    =
-    fun (self: t_FieldElement) (rhs: t_FieldElement) ->
-      let out:t_Array u64 (mk_usize 5) = Rust_primitives.Hax.repeat (mk_u64 0) (mk_usize 5) in
-      let out:t_Array u64 (mk_usize 5) =
-        Libcrux_hacl_rs.Bignum25519_51_.fadd out (self._0 <: t_Slice u64) (rhs._0 <: t_Slice u64)
-      in
-      FieldElement out <: t_FieldElement
-  }
-
-[@@ FStar.Tactics.Typeclasses.tcinstance]
-let impl_3: Core_models.Ops.Arith.t_Sub t_FieldElement t_FieldElement =
-  {
-    f_Output = t_FieldElement;
-    f_sub_pre = (fun (self: t_FieldElement) (rhs: t_FieldElement) -> true);
-    f_sub_post = (fun (self: t_FieldElement) (rhs: t_FieldElement) (out1: t_FieldElement) -> true);
-    f_sub
-    =
-    fun (self: t_FieldElement) (rhs: t_FieldElement) ->
-      let out:t_Array u64 (mk_usize 5) = Rust_primitives.Hax.repeat (mk_u64 0) (mk_usize 5) in
-      let out:t_Array u64 (mk_usize 5) =
-        Libcrux_hacl_rs.Bignum25519_51_.fsub out (self._0 <: t_Slice u64) (rhs._0 <: t_Slice u64)
-      in
-      FieldElement out <: t_FieldElement
-  }
-
-[@@ FStar.Tactics.Typeclasses.tcinstance]
-let impl_4: Core_models.Ops.Arith.t_Mul t_FieldElement u64 =
-  {
-    f_Output = t_FieldElement;
-    f_mul_pre = (fun (self: t_FieldElement) (rhs: u64) -> true);
-    f_mul_post = (fun (self: t_FieldElement) (rhs: u64) (out1: t_FieldElement) -> true);
-    f_mul
-    =
-    fun (self: t_FieldElement) (rhs: u64) ->
-      let out:t_Array u64 (mk_usize 5) = Rust_primitives.Hax.repeat (mk_u64 0) (mk_usize 5) in
-      let out:t_Array u64 (mk_usize 5) =
-        Libcrux_hacl_rs.Bignum25519_51_.fmul1 out (self._0 <: t_Slice u64) rhs
-      in
-      FieldElement out <: t_FieldElement
-  }
-
-[@@ FStar.Tactics.Typeclasses.tcinstance]
-let impl_5: Core_models.Ops.Arith.t_Mul t_FieldElement t_FieldElement =
-  {
-    f_Output = t_FieldElement;
-    f_mul_pre = (fun (self: t_FieldElement) (rhs: t_FieldElement) -> true);
-    f_mul_post = (fun (self: t_FieldElement) (rhs: t_FieldElement) (out1: t_FieldElement) -> true);
-    f_mul
-    =
-    fun (self: t_FieldElement) (rhs: t_FieldElement) ->
-      let out:t_Array u64 (mk_usize 5) = Rust_primitives.Hax.repeat (mk_u64 0) (mk_usize 5) in
-      let (tmp: t_Array u128 (mk_usize 10)):t_Array u128 (mk_usize 10) =
-        Rust_primitives.Hax.repeat (Libcrux_hacl_rs.Fstar.Uint128.uint64_to_uint128 (mk_u64 0)
-            <:
-            u128)
-          (mk_usize 10)
-      in
-      let out:t_Array u64 (mk_usize 5) =
-        Libcrux_hacl_rs.Bignum25519_51_.fmul out
-          (self._0 <: t_Slice u64)
-          (rhs._0 <: t_Slice u64)
-          (tmp <: t_Slice u128)
-      in
-      FieldElement out <: t_FieldElement
-  }
-
-let impl_17__ONE: t_FieldElement =
-  FieldElement
-  (let list = [mk_u64 1; mk_u64 0; mk_u64 0; mk_u64 0; mk_u64 0] in
-    FStar.Pervasives.assert_norm (Prims.eq2 (List.Tot.length list) 5);
-    Rust_primitives.Hax.array_of_list 5 list)
-  <:
-  t_FieldElement
-
-let impl_17__square (self: t_FieldElement) : t_FieldElement =
-  let (out: t_Array u64 (mk_usize 5)):t_Array u64 (mk_usize 5) =
-    Rust_primitives.Hax.repeat (mk_u64 0) (mk_usize 5)
-  in
-  let (tmp: t_Array u128 (mk_usize 10)):t_Array u128 (mk_usize 10) =
-    Rust_primitives.Hax.repeat (Libcrux_hacl_rs.Fstar.Uint128.uint64_to_uint128 (mk_u64 0) <: u128)
-      (mk_usize 10)
-  in
-  let out:t_Array u64 (mk_usize 5) =
-    Libcrux_hacl_rs.Bignum25519_51_.fsqr out (self._0 <: t_Slice u64) (tmp <: t_Slice u128)
-  in
-  FieldElement out <: t_FieldElement
-
-let impl_17__conditional_negate (self: t_FieldElement) (choice: Subtle.t_Choice) : t_FieldElement =
-  let neg:t_FieldElement =
-    Core_models.Ops.Arith.f_sub #t_FieldElement
-      #t_FieldElement
-      #FStar.Tactics.Typeclasses.solve
-      (Ristretto255.Traits.f_identity #t_FieldElement #FStar.Tactics.Typeclasses.solve ()
-        <:
-        t_FieldElement)
-      self
-  in
-  let mask:u64 =
-    Core_models.Num.impl_u64__wrapping_sub (mk_u64 0)
-      (cast (Subtle.impl_Choice__unwrap_u8 choice <: u8) <: u64)
-  in
-  let self:t_FieldElement =
-    Rust_primitives.Hax.Folds.fold_range (mk_usize 0)
-      (mk_usize 5)
-      (fun self temp_1_ ->
-          let self:t_FieldElement = self in
-          let _:usize = temp_1_ in
-          true)
-      self
-      (fun self i ->
-          let self:t_FieldElement = self in
-          let i:usize = i in
-          {
-            self with
-            _0
-            =
-            Rust_primitives.Hax.Monomorphized_update_at.update_at_usize self._0
-              i
-              ((self._0.[ i ] <: u64) ^.
-                (mask &. ((self._0.[ i ] <: u64) ^. (neg._0.[ i ] <: u64) <: u64) <: u64)
-                <:
-                u64)
-            <:
-            t_Array u64 (mk_usize 5)
-          }
-          <:
-          t_FieldElement)
-  in
-  self
-
-let impl_17__conditional_assign (self other: t_FieldElement) (choice: Subtle.t_Choice)
-    : t_FieldElement =
-  let mask:u64 =
-    Core_models.Num.impl_u64__wrapping_sub (mk_u64 0)
-      (cast (Subtle.impl_Choice__unwrap_u8 choice <: u8) <: u64)
-  in
-  let self:t_FieldElement =
-    Rust_primitives.Hax.Folds.fold_range (mk_usize 0)
-      (mk_usize 5)
-      (fun self temp_1_ ->
-          let self:t_FieldElement = self in
-          let _:usize = temp_1_ in
-          true)
-      self
-      (fun self i ->
-          let self:t_FieldElement = self in
-          let i:usize = i in
-          {
-            self with
-            _0
-            =
-            Rust_primitives.Hax.Monomorphized_update_at.update_at_usize self._0
-              i
-              ((self._0.[ i ] <: u64) ^.
-                (mask &. ((self._0.[ i ] <: u64) ^. (other._0.[ i ] <: u64) <: u64) <: u64)
-                <:
-                u64)
-            <:
-            t_Array u64 (mk_usize 5)
-          }
-          <:
-          t_FieldElement)
-  in
-  self
-
-let impl_17__load8_at (input: t_Array u8 (mk_usize 32)) (i: usize)
-    : Prims.Pure u64 (requires Rust_primitives.Integers.v i + 7 < 32) (fun _ -> Prims.l_True) =
-  (((((((cast (input.[ i ] <: u8) <: u64) |.
-              ((cast (input.[ i +! mk_usize 1 <: usize ] <: u8) <: u64) <<! mk_i32 8 <: u64)
-              <:
-              u64) |.
-            ((cast (input.[ i +! mk_usize 2 <: usize ] <: u8) <: u64) <<! mk_i32 16 <: u64)
-            <:
-            u64) |.
-          ((cast (input.[ i +! mk_usize 3 <: usize ] <: u8) <: u64) <<! mk_i32 24 <: u64)
-          <:
-          u64) |.
-        ((cast (input.[ i +! mk_usize 4 <: usize ] <: u8) <: u64) <<! mk_i32 32 <: u64)
-        <:
-        u64) |.
-      ((cast (input.[ i +! mk_usize 5 <: usize ] <: u8) <: u64) <<! mk_i32 40 <: u64)
+      CompressedRistretto (Rust_primitives.Hax.repeat (mk_u8 0) (mk_usize 32))
       <:
-      u64) |.
-    ((cast (input.[ i +! mk_usize 6 <: usize ] <: u8) <: u64) <<! mk_i32 48 <: u64)
-    <:
-    u64) |.
-  ((cast (input.[ i +! mk_usize 7 <: usize ] <: u8) <: u64) <<! mk_i32 56 <: u64)
+      t_CompressedRistretto
+  }
 
-/// Load a field element from the low 255 bits of a 32-byte input.
-/// This is intentionally non-canonical: it masks the top bit and does not
-/// reject inputs >= p.
-/// Adapted from the `curve25519-dalek` crate.
-let impl_17__from_bytes (bytes: t_Array u8 (mk_usize 32)) : t_FieldElement =
-  let (low_51_bit_mask: u64):u64 = mk_u64 2251799813685247 in
-  FieldElement
-  (let list =
-      [
-        (impl_17__load8_at bytes (mk_usize 0) <: u64) &. low_51_bit_mask;
-        ((impl_17__load8_at bytes (mk_usize 6) <: u64) >>! mk_i32 3 <: u64) &. low_51_bit_mask;
-        ((impl_17__load8_at bytes (mk_usize 12) <: u64) >>! mk_i32 6 <: u64) &. low_51_bit_mask;
-        ((impl_17__load8_at bytes (mk_usize 19) <: u64) >>! mk_i32 1 <: u64) &. low_51_bit_mask;
-        ((impl_17__load8_at bytes (mk_usize 24) <: u64) >>! mk_i32 12 <: u64) &. low_51_bit_mask
-      ]
-    in
-    FStar.Pervasives.assert_norm (Prims.eq2 (List.Tot.length list) 5);
-    Rust_primitives.Hax.array_of_list 5 list)
+[@@ FStar.Tactics.Typeclasses.tcinstance]
+let impl_1: Core_models.Default.t_Default t_CompressedRistretto =
+  {
+    f_default_pre = (fun (_: Prims.unit) -> true);
+    f_default_post = (fun (_: Prims.unit) (out: t_CompressedRistretto) -> true);
+    f_default
+    =
+    fun (_: Prims.unit) ->
+      Ristretto255.Traits.f_identity #t_CompressedRistretto #FStar.Tactics.Typeclasses.solve ()
+  }
+
+#push-options "--admit_smt_queries true"
+
+[@@ FStar.Tactics.Typeclasses.tcinstance]
+let impl_9: Core_models.Convert.t_TryFrom t_CompressedRistretto (t_Slice u8) =
+  {
+    f_Error = Core_models.Array.t_TryFromSliceError;
+    f_try_from_pre = (fun (slice: t_Slice u8) -> true);
+    f_try_from_post
+    =
+    (fun
+        (slice: t_Slice u8)
+        (out:
+          Core_models.Result.t_Result t_CompressedRistretto Core_models.Array.t_TryFromSliceError)
+        ->
+        true);
+    f_try_from = fun (slice: t_Slice u8) -> impl_8__from_slice slice
+  }
+
+#pop-options
+
+type t_EdwardsPoint = {
+  f_X:Ristretto255.Field.t_FieldElement;
+  f_Y:Ristretto255.Field.t_FieldElement;
+  f_Z:Ristretto255.Field.t_FieldElement;
+  f_T:Ristretto255.Field.t_FieldElement
+}
+
+type t_RistrettoPoint = | RistrettoPoint : t_EdwardsPoint -> t_RistrettoPoint
+
+let step_1_ (repr: t_CompressedRistretto)
+    : (Subtle.t_Choice & Subtle.t_Choice & Ristretto255.Field.t_FieldElement) =
+  let s:Ristretto255.Field.t_FieldElement =
+    Ristretto255.Field.impl_FieldElement__from_bytes (impl_8__as_bytes repr
+        <:
+        t_Array u8 (mk_usize 32))
+  in
+  let s_bytes_check:t_Array u8 (mk_usize 32) = Ristretto255.Field.impl_FieldElement__to_bytes s in
+  let s_encoding_is_canonical:Subtle.t_Choice =
+    Subtle.f_ct_eq #(t_Slice u8)
+      #FStar.Tactics.Typeclasses.solve
+      (s_bytes_check.[ Core_models.Ops.Range.RangeFull <: Core_models.Ops.Range.t_RangeFull ]
+        <:
+        t_Slice u8)
+      (impl_8__as_bytes repr <: t_Slice u8)
+  in
+  let s_is_negative:Subtle.t_Choice = Ristretto255.Field.impl_FieldElement__is_negative s in
+  s_encoding_is_canonical, s_is_negative, s
   <:
-  t_FieldElement
+  (Subtle.t_Choice & Subtle.t_Choice & Ristretto255.Field.t_FieldElement)
 
-/// Serialize this field element to canonical 32-byte encoding.
-/// Adapted from the `curve25519-dalek` crate.
-let impl_17__to_bytes (self: t_FieldElement)
-    : Prims.Pure (t_Array u8 (mk_usize 32))
-      Prims.l_True
-      (ensures
-        fun r ->
-          let r:t_Array u8 (mk_usize 32) = r in
-          ((r.[ mk_usize 31 ] <: u8) &. mk_u8 128 <: u8) =. mk_u8 0) =
-  let low_51_bit_mask:u64 = (mk_u64 1 <<! mk_i32 51 <: u64) -! mk_u64 1 in
-  let limbs:t_Array u64 (mk_usize 5) = self._0 in
-  let limbs:t_Array u64 (mk_usize 5) =
-    Rust_primitives.Hax.Monomorphized_update_at.update_at_usize limbs
-      (mk_usize 1)
-      ((limbs.[ mk_usize 1 ] <: u64) +! ((limbs.[ mk_usize 0 ] <: u64) >>! mk_i32 51 <: u64) <: u64)
+let step_2_ (s: Ristretto255.Field.t_FieldElement)
+    : (Subtle.t_Choice & Subtle.t_Choice & Subtle.t_Choice & t_RistrettoPoint) =
+  let one:Ristretto255.Field.t_FieldElement = Ristretto255.Field.impl_FieldElement__ONE in
+  let ss:Ristretto255.Field.t_FieldElement = Ristretto255.Field.impl_FieldElement__square s in
+  let u1:Ristretto255.Field.t_FieldElement =
+    Core_models.Ops.Arith.f_sub #Ristretto255.Field.t_FieldElement
+      #Ristretto255.Field.t_FieldElement
+      #FStar.Tactics.Typeclasses.solve
+      one
+      ss
   in
-  let limbs:t_Array u64 (mk_usize 5) =
-    Rust_primitives.Hax.Monomorphized_update_at.update_at_usize limbs
-      (mk_usize 0)
-      ((limbs.[ mk_usize 0 ] <: u64) &. low_51_bit_mask <: u64)
+  let u2:Ristretto255.Field.t_FieldElement =
+    Core_models.Ops.Arith.f_add #Ristretto255.Field.t_FieldElement
+      #Ristretto255.Field.t_FieldElement
+      #FStar.Tactics.Typeclasses.solve
+      one
+      ss
   in
-  let limbs:t_Array u64 (mk_usize 5) =
-    Rust_primitives.Hax.Monomorphized_update_at.update_at_usize limbs
-      (mk_usize 2)
-      ((limbs.[ mk_usize 2 ] <: u64) +! ((limbs.[ mk_usize 1 ] <: u64) >>! mk_i32 51 <: u64) <: u64)
-  in
-  let limbs:t_Array u64 (mk_usize 5) =
-    Rust_primitives.Hax.Monomorphized_update_at.update_at_usize limbs
-      (mk_usize 1)
-      ((limbs.[ mk_usize 1 ] <: u64) &. low_51_bit_mask <: u64)
-  in
-  let limbs:t_Array u64 (mk_usize 5) =
-    Rust_primitives.Hax.Monomorphized_update_at.update_at_usize limbs
-      (mk_usize 3)
-      ((limbs.[ mk_usize 3 ] <: u64) +! ((limbs.[ mk_usize 2 ] <: u64) >>! mk_i32 51 <: u64) <: u64)
-  in
-  let limbs:t_Array u64 (mk_usize 5) =
-    Rust_primitives.Hax.Monomorphized_update_at.update_at_usize limbs
-      (mk_usize 2)
-      ((limbs.[ mk_usize 2 ] <: u64) &. low_51_bit_mask <: u64)
-  in
-  let limbs:t_Array u64 (mk_usize 5) =
-    Rust_primitives.Hax.Monomorphized_update_at.update_at_usize limbs
-      (mk_usize 4)
-      ((limbs.[ mk_usize 4 ] <: u64) +! ((limbs.[ mk_usize 3 ] <: u64) >>! mk_i32 51 <: u64) <: u64)
-  in
-  let limbs:t_Array u64 (mk_usize 5) =
-    Rust_primitives.Hax.Monomorphized_update_at.update_at_usize limbs
-      (mk_usize 3)
-      ((limbs.[ mk_usize 3 ] <: u64) &. low_51_bit_mask <: u64)
-  in
-  let limbs:t_Array u64 (mk_usize 5) =
-    Rust_primitives.Hax.Monomorphized_update_at.update_at_usize limbs
-      (mk_usize 0)
-      ((limbs.[ mk_usize 0 ] <: u64) +!
-        (((limbs.[ mk_usize 4 ] <: u64) >>! mk_i32 51 <: u64) *! mk_u64 19 <: u64)
-        <:
-        u64)
-  in
-  let limbs:t_Array u64 (mk_usize 5) =
-    Rust_primitives.Hax.Monomorphized_update_at.update_at_usize limbs
-      (mk_usize 4)
-      ((limbs.[ mk_usize 4 ] <: u64) &. low_51_bit_mask <: u64)
-  in
-  let limbs:t_Array u64 (mk_usize 5) =
-    Rust_primitives.Hax.Monomorphized_update_at.update_at_usize limbs
-      (mk_usize 1)
-      ((limbs.[ mk_usize 1 ] <: u64) +! ((limbs.[ mk_usize 0 ] <: u64) >>! mk_i32 51 <: u64) <: u64)
-  in
-  let limbs:t_Array u64 (mk_usize 5) =
-    Rust_primitives.Hax.Monomorphized_update_at.update_at_usize limbs
-      (mk_usize 0)
-      ((limbs.[ mk_usize 0 ] <: u64) &. low_51_bit_mask <: u64)
-  in
-  let q:u64 = ((limbs.[ mk_usize 0 ] <: u64) +! mk_u64 19 <: u64) >>! mk_i32 51 in
-  let q:u64 = ((limbs.[ mk_usize 1 ] <: u64) +! q <: u64) >>! mk_i32 51 in
-  let q:u64 = ((limbs.[ mk_usize 2 ] <: u64) +! q <: u64) >>! mk_i32 51 in
-  let q:u64 = ((limbs.[ mk_usize 3 ] <: u64) +! q <: u64) >>! mk_i32 51 in
-  let q:u64 = ((limbs.[ mk_usize 4 ] <: u64) +! q <: u64) >>! mk_i32 51 in
-  let limbs:t_Array u64 (mk_usize 5) =
-    Rust_primitives.Hax.Monomorphized_update_at.update_at_usize limbs
-      (mk_usize 0)
-      ((limbs.[ mk_usize 0 ] <: u64) +! (mk_u64 19 *! q <: u64) <: u64)
-  in
-  let limbs:t_Array u64 (mk_usize 5) =
-    Rust_primitives.Hax.Monomorphized_update_at.update_at_usize limbs
-      (mk_usize 1)
-      ((limbs.[ mk_usize 1 ] <: u64) +! ((limbs.[ mk_usize 0 ] <: u64) >>! mk_i32 51 <: u64) <: u64)
-  in
-  let limbs:t_Array u64 (mk_usize 5) =
-    Rust_primitives.Hax.Monomorphized_update_at.update_at_usize limbs
-      (mk_usize 0)
-      ((limbs.[ mk_usize 0 ] <: u64) &. low_51_bit_mask <: u64)
-  in
-  let limbs:t_Array u64 (mk_usize 5) =
-    Rust_primitives.Hax.Monomorphized_update_at.update_at_usize limbs
-      (mk_usize 2)
-      ((limbs.[ mk_usize 2 ] <: u64) +! ((limbs.[ mk_usize 1 ] <: u64) >>! mk_i32 51 <: u64) <: u64)
-  in
-  let limbs:t_Array u64 (mk_usize 5) =
-    Rust_primitives.Hax.Monomorphized_update_at.update_at_usize limbs
-      (mk_usize 1)
-      ((limbs.[ mk_usize 1 ] <: u64) &. low_51_bit_mask <: u64)
-  in
-  let limbs:t_Array u64 (mk_usize 5) =
-    Rust_primitives.Hax.Monomorphized_update_at.update_at_usize limbs
-      (mk_usize 3)
-      ((limbs.[ mk_usize 3 ] <: u64) +! ((limbs.[ mk_usize 2 ] <: u64) >>! mk_i32 51 <: u64) <: u64)
-  in
-  let limbs:t_Array u64 (mk_usize 5) =
-    Rust_primitives.Hax.Monomorphized_update_at.update_at_usize limbs
-      (mk_usize 2)
-      ((limbs.[ mk_usize 2 ] <: u64) &. low_51_bit_mask <: u64)
-  in
-  let limbs:t_Array u64 (mk_usize 5) =
-    Rust_primitives.Hax.Monomorphized_update_at.update_at_usize limbs
-      (mk_usize 4)
-      ((limbs.[ mk_usize 4 ] <: u64) +! ((limbs.[ mk_usize 3 ] <: u64) >>! mk_i32 51 <: u64) <: u64)
-  in
-  let limbs:t_Array u64 (mk_usize 5) =
-    Rust_primitives.Hax.Monomorphized_update_at.update_at_usize limbs
-      (mk_usize 3)
-      ((limbs.[ mk_usize 3 ] <: u64) &. low_51_bit_mask <: u64)
-  in
-  let limbs:t_Array u64 (mk_usize 5) =
-    Rust_primitives.Hax.Monomorphized_update_at.update_at_usize limbs
-      (mk_usize 4)
-      ((limbs.[ mk_usize 4 ] <: u64) &. low_51_bit_mask <: u64)
-  in
-  let s:t_Array u8 (mk_usize 32) = Rust_primitives.Hax.repeat (mk_u8 0) (mk_usize 32) in
-  let s:t_Array u8 (mk_usize 32) =
-    Rust_primitives.Hax.Monomorphized_update_at.update_at_usize s
-      (mk_usize 0)
-      (cast (limbs.[ mk_usize 0 ] <: u64) <: u8)
-  in
-  let s:t_Array u8 (mk_usize 32) =
-    Rust_primitives.Hax.Monomorphized_update_at.update_at_usize s
-      (mk_usize 1)
-      (cast ((limbs.[ mk_usize 0 ] <: u64) >>! mk_i32 8 <: u64) <: u8)
-  in
-  let s:t_Array u8 (mk_usize 32) =
-    Rust_primitives.Hax.Monomorphized_update_at.update_at_usize s
-      (mk_usize 2)
-      (cast ((limbs.[ mk_usize 0 ] <: u64) >>! mk_i32 16 <: u64) <: u8)
-  in
-  let s:t_Array u8 (mk_usize 32) =
-    Rust_primitives.Hax.Monomorphized_update_at.update_at_usize s
-      (mk_usize 3)
-      (cast ((limbs.[ mk_usize 0 ] <: u64) >>! mk_i32 24 <: u64) <: u8)
-  in
-  let s:t_Array u8 (mk_usize 32) =
-    Rust_primitives.Hax.Monomorphized_update_at.update_at_usize s
-      (mk_usize 4)
-      (cast ((limbs.[ mk_usize 0 ] <: u64) >>! mk_i32 32 <: u64) <: u8)
-  in
-  let s:t_Array u8 (mk_usize 32) =
-    Rust_primitives.Hax.Monomorphized_update_at.update_at_usize s
-      (mk_usize 5)
-      (cast ((limbs.[ mk_usize 0 ] <: u64) >>! mk_i32 40 <: u64) <: u8)
-  in
-  let s:t_Array u8 (mk_usize 32) =
-    Rust_primitives.Hax.Monomorphized_update_at.update_at_usize s
-      (mk_usize 6)
-      (cast (((limbs.[ mk_usize 0 ] <: u64) >>! mk_i32 48 <: u64) |.
-            ((limbs.[ mk_usize 1 ] <: u64) <<! mk_i32 3 <: u64)
-            <:
-            u64)
-        <:
-        u8)
-  in
-  let s:t_Array u8 (mk_usize 32) =
-    Rust_primitives.Hax.Monomorphized_update_at.update_at_usize s
-      (mk_usize 7)
-      (cast ((limbs.[ mk_usize 1 ] <: u64) >>! mk_i32 5 <: u64) <: u8)
-  in
-  let s:t_Array u8 (mk_usize 32) =
-    Rust_primitives.Hax.Monomorphized_update_at.update_at_usize s
-      (mk_usize 8)
-      (cast ((limbs.[ mk_usize 1 ] <: u64) >>! mk_i32 13 <: u64) <: u8)
-  in
-  let s:t_Array u8 (mk_usize 32) =
-    Rust_primitives.Hax.Monomorphized_update_at.update_at_usize s
-      (mk_usize 9)
-      (cast ((limbs.[ mk_usize 1 ] <: u64) >>! mk_i32 21 <: u64) <: u8)
-  in
-  let s:t_Array u8 (mk_usize 32) =
-    Rust_primitives.Hax.Monomorphized_update_at.update_at_usize s
-      (mk_usize 10)
-      (cast ((limbs.[ mk_usize 1 ] <: u64) >>! mk_i32 29 <: u64) <: u8)
-  in
-  let s:t_Array u8 (mk_usize 32) =
-    Rust_primitives.Hax.Monomorphized_update_at.update_at_usize s
-      (mk_usize 11)
-      (cast ((limbs.[ mk_usize 1 ] <: u64) >>! mk_i32 37 <: u64) <: u8)
-  in
-  let s:t_Array u8 (mk_usize 32) =
-    Rust_primitives.Hax.Monomorphized_update_at.update_at_usize s
-      (mk_usize 12)
-      (cast (((limbs.[ mk_usize 1 ] <: u64) >>! mk_i32 45 <: u64) |.
-            ((limbs.[ mk_usize 2 ] <: u64) <<! mk_i32 6 <: u64)
-            <:
-            u64)
-        <:
-        u8)
-  in
-  let s:t_Array u8 (mk_usize 32) =
-    Rust_primitives.Hax.Monomorphized_update_at.update_at_usize s
-      (mk_usize 13)
-      (cast ((limbs.[ mk_usize 2 ] <: u64) >>! mk_i32 2 <: u64) <: u8)
-  in
-  let s:t_Array u8 (mk_usize 32) =
-    Rust_primitives.Hax.Monomorphized_update_at.update_at_usize s
-      (mk_usize 14)
-      (cast ((limbs.[ mk_usize 2 ] <: u64) >>! mk_i32 10 <: u64) <: u8)
-  in
-  let s:t_Array u8 (mk_usize 32) =
-    Rust_primitives.Hax.Monomorphized_update_at.update_at_usize s
-      (mk_usize 15)
-      (cast ((limbs.[ mk_usize 2 ] <: u64) >>! mk_i32 18 <: u64) <: u8)
-  in
-  let s:t_Array u8 (mk_usize 32) =
-    Rust_primitives.Hax.Monomorphized_update_at.update_at_usize s
-      (mk_usize 16)
-      (cast ((limbs.[ mk_usize 2 ] <: u64) >>! mk_i32 26 <: u64) <: u8)
-  in
-  let s:t_Array u8 (mk_usize 32) =
-    Rust_primitives.Hax.Monomorphized_update_at.update_at_usize s
-      (mk_usize 17)
-      (cast ((limbs.[ mk_usize 2 ] <: u64) >>! mk_i32 34 <: u64) <: u8)
-  in
-  let s:t_Array u8 (mk_usize 32) =
-    Rust_primitives.Hax.Monomorphized_update_at.update_at_usize s
-      (mk_usize 18)
-      (cast ((limbs.[ mk_usize 2 ] <: u64) >>! mk_i32 42 <: u64) <: u8)
-  in
-  let s:t_Array u8 (mk_usize 32) =
-    Rust_primitives.Hax.Monomorphized_update_at.update_at_usize s
-      (mk_usize 19)
-      (cast (((limbs.[ mk_usize 2 ] <: u64) >>! mk_i32 50 <: u64) |.
-            ((limbs.[ mk_usize 3 ] <: u64) <<! mk_i32 1 <: u64)
-            <:
-            u64)
-        <:
-        u8)
-  in
-  let s:t_Array u8 (mk_usize 32) =
-    Rust_primitives.Hax.Monomorphized_update_at.update_at_usize s
-      (mk_usize 20)
-      (cast ((limbs.[ mk_usize 3 ] <: u64) >>! mk_i32 7 <: u64) <: u8)
-  in
-  let s:t_Array u8 (mk_usize 32) =
-    Rust_primitives.Hax.Monomorphized_update_at.update_at_usize s
-      (mk_usize 21)
-      (cast ((limbs.[ mk_usize 3 ] <: u64) >>! mk_i32 15 <: u64) <: u8)
-  in
-  let s:t_Array u8 (mk_usize 32) =
-    Rust_primitives.Hax.Monomorphized_update_at.update_at_usize s
-      (mk_usize 22)
-      (cast ((limbs.[ mk_usize 3 ] <: u64) >>! mk_i32 23 <: u64) <: u8)
-  in
-  let s:t_Array u8 (mk_usize 32) =
-    Rust_primitives.Hax.Monomorphized_update_at.update_at_usize s
-      (mk_usize 23)
-      (cast ((limbs.[ mk_usize 3 ] <: u64) >>! mk_i32 31 <: u64) <: u8)
-  in
-  let s:t_Array u8 (mk_usize 32) =
-    Rust_primitives.Hax.Monomorphized_update_at.update_at_usize s
-      (mk_usize 24)
-      (cast ((limbs.[ mk_usize 3 ] <: u64) >>! mk_i32 39 <: u64) <: u8)
-  in
-  let s:t_Array u8 (mk_usize 32) =
-    Rust_primitives.Hax.Monomorphized_update_at.update_at_usize s
-      (mk_usize 25)
-      (cast (((limbs.[ mk_usize 3 ] <: u64) >>! mk_i32 47 <: u64) |.
-            ((limbs.[ mk_usize 4 ] <: u64) <<! mk_i32 4 <: u64)
-            <:
-            u64)
-        <:
-        u8)
-  in
-  let s:t_Array u8 (mk_usize 32) =
-    Rust_primitives.Hax.Monomorphized_update_at.update_at_usize s
-      (mk_usize 26)
-      (cast ((limbs.[ mk_usize 4 ] <: u64) >>! mk_i32 4 <: u64) <: u8)
-  in
-  let s:t_Array u8 (mk_usize 32) =
-    Rust_primitives.Hax.Monomorphized_update_at.update_at_usize s
-      (mk_usize 27)
-      (cast ((limbs.[ mk_usize 4 ] <: u64) >>! mk_i32 12 <: u64) <: u8)
-  in
-  let s:t_Array u8 (mk_usize 32) =
-    Rust_primitives.Hax.Monomorphized_update_at.update_at_usize s
-      (mk_usize 28)
-      (cast ((limbs.[ mk_usize 4 ] <: u64) >>! mk_i32 20 <: u64) <: u8)
-  in
-  let s:t_Array u8 (mk_usize 32) =
-    Rust_primitives.Hax.Monomorphized_update_at.update_at_usize s
-      (mk_usize 29)
-      (cast ((limbs.[ mk_usize 4 ] <: u64) >>! mk_i32 28 <: u64) <: u8)
-  in
-  let s:t_Array u8 (mk_usize 32) =
-    Rust_primitives.Hax.Monomorphized_update_at.update_at_usize s
-      (mk_usize 30)
-      (cast ((limbs.[ mk_usize 4 ] <: u64) >>! mk_i32 36 <: u64) <: u8)
-  in
-  let s:t_Array u8 (mk_usize 32) =
-    Rust_primitives.Hax.Monomorphized_update_at.update_at_usize s
-      (mk_usize 31)
-      (cast ((limbs.[ mk_usize 4 ] <: u64) >>! mk_i32 44 <: u64) <: u8)
-  in
-  s
-
-[@@ FStar.Tactics.Typeclasses.tcinstance]
-let impl_1: Subtle.t_ConstantTimeEq t_FieldElement =
-  {
-    f_ct_eq_pre = (fun (self: t_FieldElement) (other: t_FieldElement) -> true);
-    f_ct_eq_post
-    =
-    (fun (self: t_FieldElement) (other: t_FieldElement) (out: Subtle.t_Choice) -> true);
-    f_ct_eq
-    =
-    fun (self: t_FieldElement) (other: t_FieldElement) ->
-      Subtle.f_ct_eq #(t_Slice u8)
-        #FStar.Tactics.Typeclasses.solve
-        (impl_17__to_bytes self <: t_Slice u8)
-        (impl_17__to_bytes other <: t_Slice u8)
-  }
-
-let impl_17__is_negative (self: t_FieldElement) : Subtle.t_Choice =
-  let bytes:t_Array u8 (mk_usize 32) = impl_17__to_bytes self in
-  Core_models.Convert.f_into #u8
-    #Subtle.t_Choice
-    #FStar.Tactics.Typeclasses.solve
-    ((bytes.[ mk_usize 0 ] <: u8) &. mk_u8 1 <: u8)
-
-let impl_17__is_zero (self: t_FieldElement) : Subtle.t_Choice =
-  let zero:t_Array u8 (mk_usize 32) = Rust_primitives.Hax.repeat (mk_u8 0) (mk_usize 32) in
-  let bytes:t_Array u8 (mk_usize 32) = impl_17__to_bytes self in
-  Subtle.f_ct_eq #(t_Slice u8)
-    #FStar.Tactics.Typeclasses.solve
-    (bytes <: t_Slice u8)
-    (zero <: t_Slice u8)
-
-[@@ FStar.Tactics.Typeclasses.tcinstance]
-let impl_6: Core_models.Ops.Arith.t_Add t_FieldElement t_FieldElement =
-  {
-    f_Output = t_FieldElement;
-    f_add_pre = (fun (self: t_FieldElement) (rhs: t_FieldElement) -> true);
-    f_add_post = (fun (self: t_FieldElement) (rhs: t_FieldElement) (out: t_FieldElement) -> true);
-    f_add
-    =
-    fun (self: t_FieldElement) (rhs: t_FieldElement) ->
-      Core_models.Ops.Arith.f_add #t_FieldElement
-        #t_FieldElement
-        #FStar.Tactics.Typeclasses.solve
-        self
-        rhs
-  }
-
-[@@ FStar.Tactics.Typeclasses.tcinstance]
-let impl_7: Core_models.Ops.Arith.t_Sub t_FieldElement t_FieldElement =
-  {
-    f_Output = t_FieldElement;
-    f_sub_pre = (fun (self: t_FieldElement) (rhs: t_FieldElement) -> true);
-    f_sub_post = (fun (self: t_FieldElement) (rhs: t_FieldElement) (out: t_FieldElement) -> true);
-    f_sub
-    =
-    fun (self: t_FieldElement) (rhs: t_FieldElement) ->
-      Core_models.Ops.Arith.f_sub #t_FieldElement
-        #t_FieldElement
-        #FStar.Tactics.Typeclasses.solve
-        self
-        rhs
-  }
-
-[@@ FStar.Tactics.Typeclasses.tcinstance]
-let impl_8: Core_models.Ops.Arith.t_Mul t_FieldElement t_FieldElement =
-  {
-    f_Output = t_FieldElement;
-    f_mul_pre = (fun (self: t_FieldElement) (rhs: t_FieldElement) -> true);
-    f_mul_post = (fun (self: t_FieldElement) (rhs: t_FieldElement) (out: t_FieldElement) -> true);
-    f_mul
-    =
-    fun (self: t_FieldElement) (rhs: t_FieldElement) ->
-      Core_models.Ops.Arith.f_mul #t_FieldElement
-        #t_FieldElement
-        #FStar.Tactics.Typeclasses.solve
-        self
-        rhs
-  }
-
-/// Raise this field element to the power (p-5)/8 = 2^252 - 3.
-let impl_17__pow_p58 (self: t_FieldElement) : t_FieldElement =
-  let acc:t_FieldElement = impl_17__ONE in
-  let acc:t_FieldElement =
-    Core_models.Iter.Traits.Iterator.f_fold (Core_models.Iter.Traits.Collect.f_into_iter #(Core_models.Iter.Adapters.Rev.t_Rev
-            (Core_models.Ops.Range.t_Range i32))
+  let u2_sqr:Ristretto255.Field.t_FieldElement = Ristretto255.Field.impl_FieldElement__square u2 in
+  let v:Ristretto255.Field.t_FieldElement =
+    Core_models.Ops.Arith.f_sub #Ristretto255.Field.t_FieldElement
+      #Ristretto255.Field.t_FieldElement
+      #FStar.Tactics.Typeclasses.solve
+      (Core_models.Ops.Arith.f_mul #Ristretto255.Field.t_FieldElement
+          #Ristretto255.Field.t_FieldElement
           #FStar.Tactics.Typeclasses.solve
-          (Core_models.Iter.Traits.Iterator.f_rev #(Core_models.Ops.Range.t_Range i32)
+          (Core_models.Ops.Arith.f_neg #Ristretto255.Field.t_FieldElement
               #FStar.Tactics.Typeclasses.solve
-              ({
-                  Core_models.Ops.Range.f_start = mk_i32 0;
-                  Core_models.Ops.Range.f_end = mk_i32 252
-                }
-                <:
-                Core_models.Ops.Range.t_Range i32)
+              Ristretto255.Constants.v_EDWARDS_D
             <:
-            Core_models.Iter.Adapters.Rev.t_Rev (Core_models.Ops.Range.t_Range i32))
+            Ristretto255.Field.t_FieldElement)
+          (Ristretto255.Field.impl_FieldElement__square u1 <: Ristretto255.Field.t_FieldElement)
         <:
-        Core_models.Iter.Adapters.Rev.t_Rev (Core_models.Ops.Range.t_Range i32))
-      acc
-      (fun acc i ->
-          let acc:t_FieldElement = acc in
-          let i:i32 = i in
-          let acc:t_FieldElement = impl_17__square acc in
-          if i <>. mk_i32 1
-          then
-            let acc:t_FieldElement =
-              Core_models.Ops.Arith.f_mul #t_FieldElement
-                #t_FieldElement
-                #FStar.Tactics.Typeclasses.solve
-                acc
-                self
-            in
-            acc
-          else acc)
+        Ristretto255.Field.t_FieldElement)
+      u2_sqr
   in
-  acc
+  let (ok: Subtle.t_Choice), (v_I: Ristretto255.Field.t_FieldElement) =
+    Ristretto255.Field.impl_FieldElement__invsqrt (Core_models.Ops.Arith.f_mul #Ristretto255.Field.t_FieldElement
+          #Ristretto255.Field.t_FieldElement
+          #FStar.Tactics.Typeclasses.solve
+          v
+          u2_sqr
+        <:
+        Ristretto255.Field.t_FieldElement)
+  in
+  let v_Dx:Ristretto255.Field.t_FieldElement =
+    Core_models.Ops.Arith.f_mul #Ristretto255.Field.t_FieldElement
+      #Ristretto255.Field.t_FieldElement
+      #FStar.Tactics.Typeclasses.solve
+      v_I
+      u2
+  in
+  let v_Dy:Ristretto255.Field.t_FieldElement =
+    Core_models.Ops.Arith.f_mul #Ristretto255.Field.t_FieldElement
+      #Ristretto255.Field.t_FieldElement
+      #FStar.Tactics.Typeclasses.solve
+      v_I
+      (Core_models.Ops.Arith.f_mul #Ristretto255.Field.t_FieldElement
+          #Ristretto255.Field.t_FieldElement
+          #FStar.Tactics.Typeclasses.solve
+          v_Dx
+          v
+        <:
+        Ristretto255.Field.t_FieldElement)
+  in
+  let x:Ristretto255.Field.t_FieldElement =
+    Core_models.Ops.Arith.f_mul #Ristretto255.Field.t_FieldElement
+      #Ristretto255.Field.t_FieldElement
+      #FStar.Tactics.Typeclasses.solve
+      (Core_models.Ops.Arith.f_add #Ristretto255.Field.t_FieldElement
+          #Ristretto255.Field.t_FieldElement
+          #FStar.Tactics.Typeclasses.solve
+          s
+          s
+        <:
+        Ristretto255.Field.t_FieldElement)
+      v_Dx
+  in
+  let x_neg:Subtle.t_Choice = Ristretto255.Field.impl_FieldElement__is_negative x in
+  let x:Ristretto255.Field.t_FieldElement =
+    Ristretto255.Field.impl_FieldElement__conditional_negate x x_neg
+  in
+  let y:Ristretto255.Field.t_FieldElement =
+    Core_models.Ops.Arith.f_mul #Ristretto255.Field.t_FieldElement
+      #Ristretto255.Field.t_FieldElement
+      #FStar.Tactics.Typeclasses.solve
+      u1
+      v_Dy
+  in
+  let t:Ristretto255.Field.t_FieldElement =
+    Core_models.Ops.Arith.f_mul #Ristretto255.Field.t_FieldElement
+      #Ristretto255.Field.t_FieldElement
+      #FStar.Tactics.Typeclasses.solve
+      x
+      y
+  in
+  ok,
+  Ristretto255.Field.impl_FieldElement__is_negative t,
+  Ristretto255.Field.impl_FieldElement__is_zero y,
+  (RistrettoPoint ({ f_X = x; f_Y = y; f_Z = one; f_T = t } <: t_EdwardsPoint) <: t_RistrettoPoint)
+  <:
+  (Subtle.t_Choice & Subtle.t_Choice & Subtle.t_Choice & t_RistrettoPoint)
 
-[@@ FStar.Tactics.Typeclasses.tcinstance]
-let impl_9: Core_models.Ops.Arith.t_Neg t_FieldElement =
-  {
-    f_Output = t_FieldElement;
-    f_neg_pre = (fun (self: t_FieldElement) -> true);
-    f_neg_post = (fun (self: t_FieldElement) (out: t_FieldElement) -> true);
-    f_neg
-    =
-    fun (self: t_FieldElement) ->
-      Core_models.Ops.Arith.f_sub #t_FieldElement
-        #t_FieldElement
-        #FStar.Tactics.Typeclasses.solve
-        (Ristretto255.Traits.f_identity #t_FieldElement #FStar.Tactics.Typeclasses.solve ()
-          <:
-          t_FieldElement)
-        self
-  }
-
-[@@ FStar.Tactics.Typeclasses.tcinstance]
-let impl_10: Core_models.Ops.Arith.t_Neg t_FieldElement =
-  {
-    f_Output = t_FieldElement;
-    f_neg_pre = (fun (self: t_FieldElement) -> true);
-    f_neg_post = (fun (self: t_FieldElement) (out: t_FieldElement) -> true);
-    f_neg
-    =
-    fun (self: t_FieldElement) ->
-      Core_models.Ops.Arith.f_neg #t_FieldElement #FStar.Tactics.Typeclasses.solve self
-  }
-
-/// Given `FieldElements` `u` and `v`, compute either `sqrt(u/v)`
-/// or `sqrt(i*u/v)` in constant time.
-/// This function always returns the nonnegative square root.
+/// Attempt to decompress to an `RistrettoPoint`.
 /// # Return
-/// - `(Choice(1), +sqrt(u/v))  ` if `v` is nonzero and `u/v` is square;
-/// - `(Choice(1), zero)        ` if `u` is zero;
-/// - `(Choice(0), zero)        ` if `v` is zero and `u` is nonzero;
-/// - `(Choice(0), +sqrt(i*u/v))` if `u/v` is nonsquare (so `i*u/v` is square).
-let impl_17__sqrt_ratio_i (u v: t_FieldElement) : (Subtle.t_Choice & t_FieldElement) =
-  let v3:t_FieldElement =
-    Core_models.Ops.Arith.f_mul #t_FieldElement
-      #t_FieldElement
+/// - `Some(RistrettoPoint)` if `self` was the canonical encoding of a point;
+/// - `None` if `self` was not the canonical encoding of a point.
+let impl_8__decompress (self: t_CompressedRistretto) : Core_models.Option.t_Option t_RistrettoPoint =
+  let
+  (s_encoding_is_canonical: Subtle.t_Choice),
+  (s_is_negative: Subtle.t_Choice),
+  (s: Ristretto255.Field.t_FieldElement) =
+    step_1_ self
+  in
+  if
+    Core_models.Convert.f_into #Subtle.t_Choice
+      #bool
       #FStar.Tactics.Typeclasses.solve
-      (impl_17__square v <: t_FieldElement)
-      v
-  in
-  let v7:t_FieldElement =
-    Core_models.Ops.Arith.f_mul #t_FieldElement
-      #t_FieldElement
-      #FStar.Tactics.Typeclasses.solve
-      (impl_17__square v3 <: t_FieldElement)
-      v
-  in
-  let r:t_FieldElement =
-    Core_models.Ops.Arith.f_mul #t_FieldElement
-      #t_FieldElement
-      #FStar.Tactics.Typeclasses.solve
-      (Core_models.Ops.Arith.f_mul #t_FieldElement
-          #t_FieldElement
-          #FStar.Tactics.Typeclasses.solve
-          u
-          v3
-        <:
-        t_FieldElement)
-      (impl_17__pow_p58 (Core_models.Ops.Arith.f_mul #t_FieldElement
-              #t_FieldElement
-              #FStar.Tactics.Typeclasses.solve
-              u
-              v7
-            <:
-            t_FieldElement)
-        <:
-        t_FieldElement)
-  in
-  let check:t_FieldElement =
-    Core_models.Ops.Arith.f_mul #t_FieldElement
-      #t_FieldElement
-      #FStar.Tactics.Typeclasses.solve
-      v
-      (impl_17__square r <: t_FieldElement)
-  in
-  let i:t_FieldElement = v_SQRT_M1 in
-  let correct_sign_sqrt:Subtle.t_Choice =
-    Subtle.f_ct_eq #t_FieldElement #FStar.Tactics.Typeclasses.solve check u
-  in
-  let flipped_sign_sqrt:Subtle.t_Choice =
-    Subtle.f_ct_eq #t_FieldElement
-      #FStar.Tactics.Typeclasses.solve
-      check
-      (Core_models.Ops.Arith.f_neg #t_FieldElement #FStar.Tactics.Typeclasses.solve u
-        <:
-        t_FieldElement)
-  in
-  let flipped_sign_sqrt_i:Subtle.t_Choice =
-    Subtle.f_ct_eq #t_FieldElement
-      #FStar.Tactics.Typeclasses.solve
-      check
-      (Core_models.Ops.Arith.f_mul #t_FieldElement
-          #t_FieldElement
-          #FStar.Tactics.Typeclasses.solve
-          (Core_models.Ops.Arith.f_neg #t_FieldElement #FStar.Tactics.Typeclasses.solve u
-            <:
-            t_FieldElement)
-          i
-        <:
-        t_FieldElement)
-  in
-  let r_prime:t_FieldElement =
-    Core_models.Ops.Arith.f_mul #t_FieldElement
-      #t_FieldElement
-      #FStar.Tactics.Typeclasses.solve
-      v_SQRT_M1
-      r
-  in
-  let r:t_FieldElement =
-    impl_17__conditional_assign r
-      r_prime
       (Core_models.Ops.Bit.f_bitor #Subtle.t_Choice
           #Subtle.t_Choice
           #FStar.Tactics.Typeclasses.solve
-          flipped_sign_sqrt
-          flipped_sign_sqrt_i
+          (~.s_encoding_is_canonical <: Subtle.t_Choice)
+          s_is_negative
         <:
         Subtle.t_Choice)
-  in
-  let r_is_negative:Subtle.t_Choice = impl_17__is_negative r in
-  let r:t_FieldElement = impl_17__conditional_negate r r_is_negative in
-  let was_nonzero_square:Subtle.t_Choice =
-    Core_models.Ops.Bit.f_bitor #Subtle.t_Choice
-      #Subtle.t_Choice
-      #FStar.Tactics.Typeclasses.solve
-      correct_sign_sqrt
-      flipped_sign_sqrt
-  in
-  was_nonzero_square, r <: (Subtle.t_Choice & t_FieldElement)
-
-/// Attempt to compute `sqrt(1/self)` in constant time.
-/// Convenience wrapper around `sqrt_ratio_i`.
-/// This function always returns the nonnegative square root.
-/// # Return
-/// - `(Choice(1), +sqrt(1/self))  ` if `self` is a nonzero square;
-/// - `(Choice(0), zero)           ` if `self` is zero;
-/// - `(Choice(0), +sqrt(i/self))  ` if `self` is a nonzero nonsquare;
-let impl_17__invsqrt (self: t_FieldElement) : (Subtle.t_Choice & t_FieldElement) =
-  impl_17__sqrt_ratio_i impl_17__ONE self
+  then Core_models.Option.Option_None <: Core_models.Option.t_Option t_RistrettoPoint
+  else
+    let
+    (ok: Subtle.t_Choice),
+    (tt_is_negative: Subtle.t_Choice),
+    (y_is_zero: Subtle.t_Choice),
+    (res: t_RistrettoPoint) =
+      step_2_ s
+    in
+    if
+      Core_models.Convert.f_into #Subtle.t_Choice
+        #bool
+        #FStar.Tactics.Typeclasses.solve
+        (Core_models.Ops.Bit.f_bitor #Subtle.t_Choice
+            #Subtle.t_Choice
+            #FStar.Tactics.Typeclasses.solve
+            (Core_models.Ops.Bit.f_bitor #Subtle.t_Choice
+                #Subtle.t_Choice
+                #FStar.Tactics.Typeclasses.solve
+                (~.ok <: Subtle.t_Choice)
+                tt_is_negative
+              <:
+              Subtle.t_Choice)
+            y_is_zero
+          <:
+          Subtle.t_Choice)
+    then Core_models.Option.Option_None <: Core_models.Option.t_Option t_RistrettoPoint
+    else Core_models.Option.Option_Some res <: Core_models.Option.t_Option t_RistrettoPoint
